A new attempt, where W_s is still a Finset, but defined by an auxillary W_sList

FormalizationOfComputability/Phi.lean
@@ -62,20 +62,18 @@ lemma encode_ofNatCode : ∀ n, encodeCode (ofNatCode n) = n
     let m := n.div2.div2
     have hm : m < n + 4 := by
       simp only [m, div2_val]
-      exact
-        lt_of_le_of_lt (le_trans (div_le_self _ _) (div_le_self _ _))
-          (succ_le_succ (le_add_right _ _))
+      omega
     have _m1 : m.unpair.1 < n + 4 := lt_of_le_of_lt m.unpair_left_le hm
     have _m2 : m.unpair.2 < n + 4 := lt_of_le_of_lt m.unpair_right_le hm
-    have IH := encode_ofNatCode m
-    have IH1 := encode_ofNatCode m.unpair.1
-    have IH2 := encode_ofNatCode m.unpair.2
     conv_rhs => rw [← bit_bodd_div2 n, ← bit_bodd_div2 n.div2]
     simp only [ofNatCode.eq_5]
-    cases n.bodd <;> cases n.div2.bodd <;>
-      simp [m, encodeCode, IH, IH1, IH2, bit_val]
+    cases n.bodd
+    <;> cases n.div2.bodd
+    <;> simp [m, encodeCode, (encode_ofNatCode m), encode_ofNatCode m.unpair.1,
+        encode_ofNatCode m.unpair.2, bit_val]
 
 variable {e s t n x y : ℕ} {X : Set ℕ}
+
 
 /- ϕₑ,ₛ(n), the eth Turing program evaluated for s steps on input n.
 Following Soare, we require the index, input, and output to be less than s -/
@@ -88,6 +86,7 @@ def ϕ_s (e s n : ℕ) : Option ℕ :=
 def ϕ (e : ℕ) : ℕ →. ℕ := eval (ofNatCode e)
 
 /- ϕₑ,ₛ(n)↓ iff it has an output -/
+@[grind, simp]
 def ϕ_s_halts (e s n : ℕ) : Prop := (ϕ_s e s n).isSome
 
 /- ϕₑ(n)↓ iff it has an output -/
@@ -154,60 +153,26 @@ open Primrec
 
 -- a helper lemma for showing that ϕ_s is primitive recursive
 private lemma bounded_exists (f : ℕ → ℕ → Prop) (s : ℕ) [DecidableRel f]
-  (hf : PrimrecRel f) :
-    PrimrecPred (λ n => ∃ y < s, (f y n)) := by
-    replace hf := PrimrecRel.exists_mem_list hf
-    unfold PrimrecRel at hf
+    (hf : PrimrecRel f) :
+      PrimrecPred (λ n => ∃ y < s, (f y n)) := by
+    have h := PrimrecRel.exists_mem_list hf
+    unfold PrimrecRel at h
     have hpair : Primrec (λ n : ℕ => (List.range s, n)) :=
       (Primrec.const (List.range s)).pair Primrec.id
-    replace hf := hf.comp hpair
+    have h3 := h.comp hpair
     simp_all only [List.mem_range]
 
-private lemma bounded_exists_var
-    (f : ℕ → ℕ × ℕ → Prop) [DecidableRel f]
-    (hf : PrimrecRel f) :
-    PrimrecPred (fun x : ℕ × ℕ => ∃ y < x.1, f y x) := by
-  replace hf := PrimrecRel.exists_mem_list hf
-  unfold PrimrecRel at hf
-  have hpair : Primrec (fun x : ℕ × ℕ => (List.range x.1, x)) := by
-    exact (Primrec.list_range.comp Primrec.fst).pair Primrec.id
-  replace hf := hf.comp hpair
-  simpa only [List.mem_range] using hf
-
 /- ϕₑ,ₛ is a primitive recursive function -/
-lemma ϕ_s_primrec : Primrec₂ (ϕ_s e) := by
-  unfold Primrec₂
-  have h := primrec_evaln.comp (pair (pair fst (const (ofNatCode e))) snd)
-  apply ite (PrimrecPred.and (PrimrecRel.comp nat_lt (const e) fst) ?_) h (const Option.none)
-  apply bounded_exists_var
+lemma ϕ_s_primrec : Primrec (ϕ_s e s) := by
+  have h := primrec_evaln.comp (pair (pair (const s) (const (ofNatCode e))) .id)
+  apply ite (PrimrecPred.and (PrimrecRel.comp nat_lt (const e) (const s)) ?_) h (const Option.none)
+  apply bounded_exists
   simp only [PrimrecRel, Option.mem_def]
   exact PrimrecRel.comp Primrec.eq (.comp h snd) (option_some_iff.mpr fst)
 
--- /- ϕₑ,ₛ is a primitive recursive function -/
--- lemma ϕ_s_primrec' : Primrec (ϕ_s e s) := by
---   have h := primrec_evaln.comp (pair (pair (const s) (const (ofNatCode e))) .id)
---   apply ite (PrimrecPred.and (PrimrecRel.comp nat_lt (const e) (const s)) ?_) h (const Option.none)
---   apply bounded_exists
---   simp only [PrimrecRel, Option.mem_def]
---   exact PrimrecRel.comp Primrec.eq (.comp h snd) (option_some_iff.mpr fst)
-
--- /- ϕ_s_halts is a primitive recursive predicate -/
--- lemma ϕ_s_halts_primrec : PrimrecPred (ϕ_s_halts e s) := by
---   have h (n : ℕ) : (∃ x, ϕ_s e s n = some x) ↔ (∃ x < s, ϕ_s e s n = some x) := by
---     constructor
---     · intro ⟨x, h⟩
---       use x
---       simp only [ϕ_output_bound h, h, and_self]
---     · simp_all
---   unfold ϕ_s_halts
---   simp only [Option.isSome_iff_exists, h]
---   apply bounded_exists
---   apply PrimrecRel.comp₂ Primrec.eq (comp₂ (ϕ_s_primrec) (Primrec₂.right))
---   exact comp₂ option_some Primrec₂.left
-
-lemma ϕ_s_halts_primrec (e : ℕ) :
-    PrimrecPred fun (s, n) => ϕ_s_halts e s n := by
-  have h (s n : ℕ) : (∃ x, ϕ_s e s n = some x) ↔ (∃ x < s, ϕ_s e s n = some x) := by
+/- ϕ_s_halts is a primitive recursive predicate -/
+lemma ϕ_s_halts_primrec : PrimrecPred (ϕ_s_halts e s) := by
+  have h (n : ℕ) : (∃ x, ϕ_s e s n = some x) ↔ (∃ x < s, ϕ_s e s n = some x) := by
     constructor
     · intro ⟨x, h⟩
       use x
@@ -215,24 +180,17 @@ lemma ϕ_s_halts_primrec (e : ℕ) :
     · simp_all
   unfold ϕ_s_halts
   simp only [Option.isSome_iff_exists, h]
-  apply bounded_exists_var
-  refine PrimrecRel.comp₂ Primrec.eq ?_ (Primrec₂.option_some_iff.mpr Primrec₂.left)
-  refine Primrec₂.comp₂ ϕ_s_primrec (comp₂ fst Primrec₂.right) (comp₂ snd Primrec₂.right)
-
-lemma ϕ_s_halts_primrecRel (e : ℕ) :
-    PrimrecRel (fun n s : ℕ => ϕ_s_halts e s n) := by
-  unfold ϕ_s_halts
-  apply Primrec.primrecPred
-  simpa [Option.isSome_iff_exists] using
-    Primrec.option_isSome.comp ((ϕ_s_primrec (e := e)).comp snd fst)
+  apply bounded_exists
+  apply PrimrecRel.comp₂ Primrec.eq (comp₂ (ϕ_s_primrec) (Primrec₂.right))
+  exact comp₂ option_some Primrec₂.left
 
 /- ϕₑ,ₛ(n) is decidable -/
-instance ϕ_s_dec (e s n : ℕ) : Decidable (ϕ_s e s n).isSome :=
+instance (e s n : ℕ) : Decidable (ϕ_s e s n).isSome :=
   (ϕ_s e s n).isSome.decEq true
 
 /- ϕₑ,ₛ(n) is decidable -/
-instance ϕ_s_halts_dec (e s n : ℕ) : Decidable (ϕ_s_halts e s n) := by
-  exact ϕ_s_dec e s n
+instance (e s n : ℕ) : Decidable (ϕ_s_halts e s n) :=
+  instDecidableEqBoolIsSomeNatϕ_sTrue e s n
 
 /- ϕₑ is a partial computable function -/
 theorem ϕ_partrec : Nat.Partrec (ϕ e) := by
@@ -269,10 +227,11 @@ def runtime (e n : ℕ) : Part ℕ := rfind (fun s => (ϕ_s e s n).isSome)
 /- Runtime r is minimal - if s < r, then ϕₑ,ₛ(n)↑ -/
 @[simp]
 lemma runtime_spec (r : ℕ) (h : r ∈ runtime e n) : ϕ_s_halts e r n := by
-  simp_all [ϕ_s_halts]
+  simp_all only [runtime, Part.coe_some, mem_rfind, Part.mem_some_iff, Bool.true_eq, Bool.false_eq,
+    Option.isSome_eq_false_iff, Option.isNone_iff_eq_none, ϕ_s_halts]
 
 lemma runtime_min (r : ℕ) (h : r ∈ (runtime e n)) : ∀ t, t < r → ¬ ϕ_s_halts e t n := by
-  simp_all [ϕ_s_halts]
+  simp_all
 
 /- ϕₑ(n)↓ iff there is a *least* stage s at which ϕₑ,ₛ(n)↓ -/
 @[grind =, simp]
@@ -288,34 +247,30 @@ lemma ϕ_halts_runtime_exists : ϕ_halts e n ↔ ∃ r, r ∈ runtime e n := by
       exact hs
     simpa [Part.dom_iff_mem] using h1
   · intro ⟨r, h⟩
-    apply ϕ_complete.mpr
     apply runtime_spec at h
-    exact ⟨r, h⟩
+    exact ϕ_complete.mpr ⟨r, h⟩
 
 /- Wₑ,ₛ = the domain of ϕₑ,ₛ, i.e. elements entering before stage s.
 As all inputs n ≥ s do not halt, this set is necessarily finite. -/
+@[grind, simp]
+def W_sList (e s : ℕ) : List ℕ := (List.range s).filter (fun n => ϕ_s_halts e s n)
 
-def W_s (e s : ℕ): List ℕ := (List.range s).filter (ϕ_s_halts e s)
-
-/- The Wₑ,ₛ are primitive recursive-/
-lemma W_s_primrec (e : ℕ) : Primrec fun (s : ℕ) => W_s e s := by
-  unfold W_s
-  have hrel : PrimrecRel (fun n s : ℕ => ϕ_s_halts e s n) :=
-    ϕ_s_halts_primrecRel e
-  exact
-    ((PrimrecRel.listFilter hrel).comp
-      Primrec.list_range
-      Primrec.id)
-
-@[grind =, simp]
-lemma W_s_mem (e s n : ℕ) : n ∈ W_s e s ↔ n < s ∧ ϕ_s_halts e s n := by
-  simp [W_s]
+@[grind, simp]
+def W_s (e s : ℕ): Finset ℕ := (W_sList e s).toFinset
 
 /- Wₑ = {n | ϕₑ(n)↓} -/
 @[grind, simp]
 def W (e : ℕ) : Set ℕ := (ϕ e).Dom
 
--- instance W_s_dec (e s n : ℕ) : Decidable (n ∈ W_s e s) := by apply Finset.decidableMem
+lemma W_s_primrec (e : ℕ) : Primrec fun (s : ℕ) ↦ W_s e s := by
+  have h0 (s) : PrimrecPred (ϕ_s_halts e s) := ϕ_s_halts_primrec
+  unfold W_s
+  sorry
+
+@[simp]
+lemma W_s_mem (e s n : ℕ) : n ∈ W_s e s ↔ ϕ_s_halts e s n := by
+  simp
+  exact fun a ↦ ϕ_input_bound a
 
 /- The Wₑ are Σ01 -/
 lemma W_Sigma01 (e : ℕ) : Sigma01 (W e) := by
@@ -347,14 +302,17 @@ lemma Sigma01_iff_W : Sigma01 X ↔ ∃ e, X = W e := by grind [Sigma01_is_W, W_
 /- ϕₑ,ₛ(n)↓ iff n ∈ Wₑ,ₛ -/
 @[simp]
 lemma W_s_ϕ_s : n ∈ W_s e s ↔ ϕ_s_halts e s n := by
-  simp_all [W_s_mem, ϕ_s_halts, and_iff_right_iff_imp]
+  simp_all only [W_s, W_sList, ϕ_s_halts, Bool.decide_eq_true, List.toFinset_filter,
+    Finset.mem_filter, List.mem_toFinset, List.mem_range, and_iff_right_iff_imp]
   exact fun a ↦ ϕ_input_bound a
 
 @[simp]
-lemma Ws_gt_zero : n ∈ W_s e s → s > 0 := by grind
+lemma Ws_gt_zero : n ∈ W_s e s → s > 0 := by
+  simp [W_s, W_sList]
+  omega
 
 @[simp]
-lemma Ws_zero_empty : W_s e 0 = ∅ := by simp [W_s]
+lemma Ws_zero_empty : W_s e 0 = ∅ := by simp [W_s, W_sList]
 
 /- ϕₑ(x)↓ ↔ x ∈ Wₑ -/
 @[simp]
@@ -362,11 +320,18 @@ lemma mem_W_ϕ : n ∈ W e ↔ ϕ_halts e n := by exact Eq.to_iff rfl
 
 /- Monotonicity of W_s: W_s ⊆ W_{e, s+1}  -/
 @[simp]
-lemma W_s_mono (h : s ≤ t) : (W_s e s) ⊆ (W_s e t) := by grind
+lemma W_s_mono (h : s ≤ t) : (W_s e s) ⊆ (W_s e t) := by
+  refine Finset.subset_iff.mpr ?_
+  intro x
+  simp only [W_s_mem]
+  exact fun a ↦ ϕ_halts_mono h a
+
 
 /- Reverse monotonicity of W_s-/
 @[simp]
-lemma W_s_mono_reverse (h : s ≤ t) (hx : x ∉ W_s e t) : x ∉ W_s e s := by grind
+lemma W_s_mono_reverse (h : s ≤ t) (hx : x ∉ W_s e t) : x ∉ W_s e s := by
+  contrapose hx
+  exact W_s_mono h hx
 
 /- Membership in some W_{e,s} implies runtime r exists, and membership in W_{e, r}-/
 @[grind ., simp]
@@ -378,19 +343,24 @@ lemma Ws_runtime (h : n ∈ W_s e s) : ∃ r, r ∈ runtime e n ∧ n ∈ W_s e 
 
 /- Wₑ,ₛ ⊆ Wₑ  -/
 @[grind! ., simp]
-lemma W_s_subset_W : ↑(W_s e s).toFinset ⊆ W e := by
+lemma W_s_subset_W : ↑(W_s e s) ⊆ W e := by
   intro x h
-  simp [W_s] at h
-  refine mem_W_ϕ.mpr (ϕ_complete.mpr ?_)
+  rw [mem_W_ϕ]
+  simp [W_s, W_sList, Finset.coe_filter, Set.mem_setOf_eq] at h
+  rw [ϕ_complete]
   use s
   simp [h.right]
 
 /- Wₑ = ⋃ₛ Wₑ,ₛ -/
 @[grind =, simp]
 lemma W_mem_iff_W_s : n ∈ W e ↔ ∃ s, n ∈ W_s e s := by
-  simp only [W_s_ϕ_s, ϕ_complete, mem_W_ϕ]
+  constructor
+  · intro h
+    simp only [W_s_ϕ_s]
+    exact ϕ_complete.mp (mem_W_ϕ.mp h)
+  · grind
 
-lemma W_eq_union_W_s : W e = ⋃ (s : ℕ), (W_s e s).toFinset := by
+lemma W_eq_union_W_s : W e = ⋃ (s : ℕ), W_s e s := by
   ext x
   rw [W_mem_iff_W_s]
   simp
